Finished pset 8

pset08_HoareLogic/Pset8.v
@@ -150,8 +150,62 @@ Open Scope reset_scope.
 
 (** * Define your semantics here! *)
 
-Axiom exec : trace -> heap -> valuation -> cmd ->
-             trace -> heap -> valuation -> Prop.
+(* Shorthand notation for looking up in a finite map, returning zero if the key
+ * is not found *)
+Notation "m $! k" := (match m $? k with Some n => n | None => O end) (at level 30).
+
+(* Start of expression semantics: meaning of expressions *)
+Fixpoint eval (e : exp) (h : heap) (v : valuation) : nat :=
+  match e with
+  | Const n => n
+  | Var x => v $! x
+  | Read e1 => h $! eval e1 h v
+  | Plus e1 e2 => eval e1 h v + eval e2 h v
+  | Minus e1 e2 => eval e1 h v - eval e2 h v
+  | Mult e1 e2 => eval e1 h v * eval e2 h v
+  end.
+
+(* Meaning of Boolean expressions *)
+Fixpoint beval (b : bexp) (h : heap) (v : valuation) : bool :=
+  match b with
+  | Equal e1 e2 => if eval e1 h v ==n eval e2 h v then true else false
+  | Less e1 e2 => if eval e2 h v <=? eval e1 h v then false else true
+  end.
+
+Inductive exec : trace ->heap -> valuation -> cmd -> trace -> heap -> valuation -> Prop :=
+| ExSkip : forall t h v,
+  exec t h v Skip t h v
+| ExAssign : forall t h v x e,
+  exec t h v (Assign x e) t h (v $+ (x, eval e h v))
+| ExWrite : forall t h v e1 e2,
+  exec t h v (Write e1 e2) t (h $+ (eval e1 h v, eval e2 h v)) v
+| ExSeq : forall t1 h1 v1 c1 t2 h2 v2 c2 t3 h3 v3,
+  exec t1 h1 v1 c1 t2 h2 v2
+  -> exec t2 h2 v2 c2 t3 h3 v3
+  -> exec t1 h1 v1 (Seq c1 c2) t3 h3 v3
+| ExIfTrue : forall t1 h1 v1 b c1 c2 t2 h2 v2,
+  beval b h1 v1 = true
+  -> exec t1 h1 v1 c1 t2 h2 v2
+  -> exec t1 h1 v1 (If_ b c1 c2) t2 h2 v2
+| ExIfFalse : forall t1 h1 v1 b c1 c2 t2 h2 v2,
+  beval b h1 v1 = false
+  -> exec t1 h1 v1 c2 t2 h2 v2
+  -> exec t1 h1 v1 (If_ b c1 c2) t2 h2 v2
+| ExWhileFalse : forall I t h v b c,
+  beval b h v = false
+  -> exec t h v (While_ I b c) t h v
+| ExWhileTrue : forall I t1 h1 v1 b c t2 h2 v2 t3 h3 v3,
+  beval b h1 v1 = true
+  -> exec t1 h1 v1 c t2 h2 v2
+  -> exec t2 h2 v2 (While_ I b c) t3 h3 v3
+  -> exec t1 h1 v1 (While_ I b c) t3 h3 v3
+| ExAssert : forall t h v (a : iassertion),
+  a h v
+  -> exec t h v (Assert a) t h v
+| ExInput : forall t h v x xv,
+  exec t h v (Input x) (In xv :: t) h (v $+ (x, xv))
+| ExOutput : forall t h v e,
+  exec t h v (Output e) (Out (eval e h v) :: t) h v.
 
 
 (** * Task 2 : Hoare logic *)
@@ -170,7 +224,44 @@ Axiom exec : trace -> heap -> valuation -> cmd ->
 
 (** Task 2-1: Define your Hoare logic here! *)
 
-Axiom hoare_triple : assertion -> cmd -> assertion -> Prop.
+Inductive hoare_triple : assertion -> cmd -> assertion -> Prop :=
+| HtSkip : forall P, hoare_triple P Skip P
+| HtAssign : forall (P : assertion) x e,
+  hoare_triple P (Assign x e) (fun t h v => exists v', P t h v' /\ v = v' $+ (x, eval e h v'))
+| HtWrite : forall (P : assertion) (e1 e2 : exp),
+  hoare_triple P (Write e1 e2) (fun t h v => exists h', P t h' v /\ h = h' $+ (eval e1 h' v, eval e2 h' v))
+| HtSeq : forall (P Q R : assertion) c1 c2,
+  hoare_triple P c1 Q
+  -> hoare_triple Q c2 R
+  -> hoare_triple P (Seq c1 c2) R
+| HtIf : forall (P Q1 Q2 : assertion) b c1 c2,
+  hoare_triple (fun t h v => P t h v /\ beval b h v = true) c1 Q1
+  -> hoare_triple (fun t h v => P t h v /\ beval b h v = false) c2 Q2
+  -> hoare_triple P (If_ b c1 c2) (fun t h v => Q1 t h v \/ Q2 t h v)
+| HtWhile : forall (I P : assertion) b c,
+  (forall t h v, P t h v -> I t h v)
+  -> hoare_triple (fun t h v => I t h v /\ beval b h v = true) c I
+  -> hoare_triple P (While_ I b c) (fun t h v => I t h v /\ beval b h v = false)
+| HtAssert : forall (P : assertion) (I : iassertion),
+  (forall t h v, P t h v -> I h v)
+  -> hoare_triple P (Assert I) P
+| HtConsequence : forall (P Q P' Q' : assertion) c,
+  hoare_triple P c Q
+  -> (forall t h v, P' t h v -> P t h v)
+  -> (forall t h v, Q t h v -> Q' t h v)
+  -> hoare_triple P' c Q'
+| HtInput : forall (P : assertion) x,
+  hoare_triple P (Input x) (fun t h v => exists xv v' t', P t' h v' /\ v = v' $+ (x, xv) /\ t = (In xv :: t'))
+| HtOutput : forall (P : assertion) (e : exp),
+  hoare_triple P (Output e) (fun t h v => exists t', P t' h v /\ t = (Out (eval e h v) :: t')).
+
+Lemma HtStrengthenPost : forall (P Q Q' : assertion) c,
+  hoare_triple P c Q
+  -> (forall t h v, Q t h v -> Q' t h v)
+  -> hoare_triple P c Q'.
+Proof.
+  simplify; eapply HtConsequence; eauto.
+Qed.
 
 Notation "[[ tr , h , v ]] ~> e" := (fun tr h v => e%reset) (at level 90).
 Notation "{{ P }} c {{ Q }}" :=
@@ -178,14 +269,34 @@ Notation "{{ P }} c {{ Q }}" :=
 
 (** Task 2-2: Prove the consistency theorem. *)
 
+(* Let's prove that the intuitive description given above really applies to this
+ * predicate.  First, a lemma, which is difficult to summarize intuitively!
+ * More or less precisely this obligation shows up in the main proof below. *)
+Lemma hoare_triple_big_step_while: forall (I : assertion) b c,
+  (forall t h v t' h' v', exec t h v c t' h' v'
+                     -> I t h v
+                     -> beval b h v = true
+                     -> I t' h' v')
+  -> forall t h v t' h' v', exec t h v (While_ I b c) t' h' v'
+                       -> I t h v
+                       -> I t' h' v' /\ beval b h' v' = false.
+Proof.
+  induct 2; eauto.
+Qed.
+
 Theorem hoare_triple_big_step :
   forall pre c post,
     hoare_triple pre c post ->
-    forall tr h v tr' h' v',
-      exec tr h v c tr' h' v' ->
-      pre tr h v -> post tr' h' v'.
+    forall t h v t' h' v',
+      exec t h v c t' h' v' ->
+      pre t h v -> post t' h' v'.
 Proof.
-Admitted.
+    induct 1; eauto; invert 1; eauto; simplify.
+
+    eapply hoare_triple_big_step_while; try eauto.
+
+    exists xv. exists v. exists t. propositional.
+Qed.
 
 
 (** * Task 3: Verification of some example programs *)
@@ -209,7 +320,17 @@ Theorem add_two_inputs_ok:
     tr = nil ->
     exists vx vy, tr' = [Out (vx + vy); In vy; In vx].
 Proof.
-Admitted.
+    simplify.
+    invert H.
+    invert H6.
+    invert H10.
+    invert H4.
+    invert H8.
+    exists xv.
+    exists xv0.
+    simplify.
+    equality.
+Qed.
 
 (** Task 3-2: finding the maximum of three numbers -- prove [max3_ok] *)
 
@@ -245,9 +366,57 @@ Theorem max3_ok:
     tr = nil ->
     max3_spec tr'.
 Proof.
-Admitted.
+    simplify.
+    invert H. invert H6.
+    invert H10. invert H4.
+    invert H8. invert H4.
+
+    invert H9.
+    invert H8.
+    invert H10.
+    all: simplify; cases (xv0 <=? xv); cases (xv1 <=? xv0); try linear_arithmetic; try equality.
+    1: {
+        invert H11.
+        simplify.
+        econstructor; linear_arithmetic.
+    }
+    1: {
+        invert H11.
+        simplify.
+        econstructor; linear_arithmetic.
+    }
+    1: {
+        invert H10.
+        invert H9.
+        invert H11.
+        simplify.
+        all: simplify; cases (xv1 <=? xv); try linear_arithmetic; try equality.
+        invert H11.
+        simplify.
+        econstructor; linear_arithmetic.
+    }
+    invert H10.
+    invert H9.
+    invert H11.
+    simplify.
+    all: simplify; cases (xv1 <=? xv); try linear_arithmetic; try equality.
+    1: econstructor; linear_arithmetic.
+    invert H11.
+    simplify.
+    econstructor; linear_arithmetic.
+Qed.
 
 (** Task 3-3: Fibonacci sequence -- prove [fibonacci_ok] *)
+
+Fixpoint fib (n : nat) : nat :=
+  match n with
+  | O => 1
+  | S n' =>
+    match n' with
+    | O => 1
+    | S n'' => fib n' + fib n''
+    end
+  end.
 
 Inductive fibonacci_spec : trace -> Prop :=
 | Fs0: fibonacci_spec nil
@@ -263,8 +432,12 @@ Example fibonacci (n: nat) :=
    "x" <- 0;;
    "y" <- 1;;
    output "y";;
-   {{ fun _ _ _ => True }} (* You may change this loop invariant to make your
-                            * proof easier! *)
+   {{ [[ t , h , v ]] ~> exists t',
+       (v $! "cnt" = 0 /\ v $! "x" = 0 /\ v $! "y" = 1 /\ t = (Out 1 :: nil)) \/
+       (v $! "cnt" = 1 /\ v $! "x" = 1 /\ v $! "y" = 1 /\ t = (Out 1 :: Out 1 :: nil)) \/ 
+       (v $! "cnt" >= 2 /\ v $! "y" = fib (v $! "cnt") /\ v $! "x" = fib (v $! "cnt" - 1)
+                        /\ t = (Out (v $! "y") :: Out (v $! "x") :: t')
+                        /\ fibonacci_spec t) }}
    while "cnt" < n loop
      "tmp" <- "y";;
      "y" <- "x" + "y";;
@@ -273,25 +446,152 @@ Example fibonacci (n: nat) :=
      output "y"
    done)%cmd.
 
+Ltac invert_commands := repeat match goal with
+                               | [ H : exec _ _ _ (Seq _ _) _ _ _ |- _ ] => invert H
+                               | [ H : exec _ _ _ (Assign _ _) _ _ _ |- _ ] => invert H
+                               | [ H : exec _ _ _ (Input _) _ _ _ |- _ ] => invert H
+                               | [ H : exec _ _ _ (Output _) _ _ _ |- _ ] => invert H
+                               end; simplify.
+
+Ltac ht1 := apply HtSkip || apply HtAssign || apply HtWrite || eapply HtSeq
+            || eapply HtIf || eapply HtWhile || eapply HtAssert
+            || eapply HtInput || eapply HtOutput.
+
+Ltac t := cbv beta; propositional; subst;
+          repeat match goal with
+                 | [ H : ex _ |- _ ] => invert H; propositional; subst
+                 end;
+          simplify;
+          repeat match goal with
+                 | [ _ : context[?a <=? ?b] |- _ ] => destruct (a <=? b); try discriminate
+                 | [ H : ?E = ?E |- _ ] => clear H
+                 end; simplify; propositional; auto; try equality; try linear_arithmetic.
+
+Ltac ht := simplify; repeat ht1; t.
+
+Lemma fibonacci_ok' (n: nat): forall n,
+  {{ [[ t , h , v ]] ~> t = nil }}
+  fibonacci n
+  {{ [[ t , h , v ]] ~> exists t',
+      (v $! "cnt" = 0 /\ v $! "x" = 0 /\ v $! "y" = 1 /\ t = (Out 1 :: nil)) \/
+      (v $! "cnt" = 1 /\ v $! "x" = 1 /\ v $! "y" = 1 /\ t = (Out 1 :: Out 1 :: nil)) \/ 
+      (v $! "cnt" >= 2 /\ v $! "y" = fib (v $! "cnt") /\ v $! "x" = fib (v $! "cnt" - 1)
+                       /\ t = (Out (v $! "y") :: Out (v $! "x") :: t')
+                       /\ fibonacci_spec t) }}.
+Proof.
+  simplify.
+  eapply HtSeq; try apply HtAssign.
+  eapply HtSeq; try apply HtAssign.
+  eapply HtSeq; try apply HtAssign.
+  eapply HtSeq.
+  apply HtOutput.
+
+  eapply HtStrengthenPost.
+
+  eapply HtWhile.
+
+  1: {
+    simplify.
+    ht.
+    exists nil.
+    equality.
+  }
+
+  1: {
+    ht.
+    eapply HtStrengthenPost.
+    eapply HtOutput.
+    ht.
+    1: {
+      rewrite H; rewrite H0; rewrite H1; simplify.
+      exists (x0).
+      right.
+      left.
+      propositional.
+    }
+    1: {
+      rewrite H; rewrite H0; rewrite H1; simplify.
+      exists (Out 1 :: nil).
+      right.
+      right.
+      propositional; try linear_arithmetic.
+        replace 2 with (1 + 1); try linear_arithmetic.
+        econstructor.
+        econstructor.
+    }
+    rewrite H; rewrite H1; simplify.
+    eexists.
+    right.
+    right.
+    propositional.
+    1: linear_arithmetic.
+    1: {
+      symmetry.
+      cases (x1 $! "cnt" + 1); try linear_arithmetic.
+      assert (x1 $! "cnt" = n1); try linear_arithmetic; subst.
+      remember (x1 $! "cnt") as k.
+      assert (exists k', k = S k').
+      1: exists (k - 1); linear_arithmetic.
+      simplify.
+      invert H2.
+      cases (x1 $! "cnt"); try linear_arithmetic.
+      replace (S n1 - 1) with n1; try linear_arithmetic.
+    }
+    cases (x1 $! "cnt"); simplify; try linear_arithmetic.
+    invert H0; simplify; try linear_arithmetic.
+    cases n1; try linear_arithmetic.
+    simplify.
+    cases n1; try linear_arithmetic.
+    cases (S n1 + 1); try linear_arithmetic.
+    subst.
+    invert Heq0.
+    cases n1; try linear_arithmetic.
+    1: simplify; equality.
+    replace (S n1 + 1) with (S (S n1)); try linear_arithmetic.
+    simplify.
+    equality.
+    econstructor.
+    rewrite <- H1.
+    rewrite <- H.
+    assumption.
+  }
+
+  ht.
+Qed.
+
 Theorem fibonacci_ok (n: nat):
   forall tr h v tr' h' v',
     exec tr h v (fibonacci n) tr' h' v' ->
     tr = nil ->
     fibonacci_spec tr'.
 Proof.
-Admitted.
+  simplify.
+  eapply hoare_triple_big_step with (c := fibonacci n) (t := tr) (t' := tr'); try eassumption.
+  (*eapply hoare_triple_big_step; try eassumption.*)
+  1: {
+    eapply HtStrengthenPost.
+    1: eapply fibonacci_ok'; assumption.
+    simplify.
+    invert H1.
+    propositional; subst.
+    1: constructor.
+    1: constructor.
+  }
+  simplify.
+  assumption.
+Qed.
 
 
 (** * Task 4-1: please estimate the time you have spent on this pset so far:
 
-  space for work provided here (not graded):
+  space for work provided here (not graded): 14
 
 *)
 
 (** * Task 4-2: please subtract the answer of 4-1 from 8 hours:
    (8 hours is our target time when designing these psets):
 
-  space for work provided here (not graded):
+  space for work provided here (not graded): 6
 
 *)
 
@@ -312,3 +612,77 @@ Admitted.
  *)
 
 (** Define your own program and prove its correctness here! *)
+
+Example index_in_3_inputs :=
+  ( "n0" <-- input;;
+    "n1" <-- input;;
+    "n2" <-- input;;
+    *[0] <- "n0";;
+    *[1] <- "n1";;
+    *[2] <- "n2";;
+    "index" <-- input;;
+    output *["index"]
+  )%cmd.
+
+Inductive index_spec : trace -> Prop :=
+| Index0: forall n0 n1 n2, index_spec [Out n0; In 0; In n2; In n1; In n0]
+| Index1: forall n0 n1 n2, index_spec [Out n1; In 1; In n2; In n1; In n0]
+| Index2: forall n0 n1 n2, index_spec [Out n2; In 2; In n2; In n1; In n0]
+| Index_invalid: forall  t index, index > 2 -> index_spec t.
+
+Theorem index_ok (n: nat):
+  forall t h v t' h' v',
+    exec t h v index_in_3_inputs t' h' v' ->
+    t = nil ->
+    index_spec t'.
+Proof.
+  simplify.
+  invert H.
+  repeat match goal with
+         | [ H : exec _ _ _ _ _ _ _ |- _ ] => invert H
+         end; invert_commands; simplify.
+  cases xv; simplify; try econstructor; cases xv; simplify; econstructor.
+Qed.
+
+(*Example add_n_inputs :=*)
+  (*( "n" <-- input;;*)
+    (*"cnt" <- 0;;*)
+    (*"sum" <- 0;;*)
+    (*{{ [[ t , h , v ]] ~> True }}*)
+    (*while "cnt" < "n" loop*)
+      (*"tmp" <-- input;;*)
+      (**["cnt"] <- "tmp";;*)
+      (*"cnt" <- "cnt" + 1*)
+    (*done;;*)
+    (*"cnt" <- 0;;*)
+    (*{{ [[ t , h , v ]] ~> True }}*)
+    (*while "cnt" < "n" loop*)
+      (*"sum" <- "sum" + *["cnt"]*)
+    (*done;;*)
+    (*output "sum"*)
+  (*)%cmd.*)
+
+(*Fixpoint sum_spec (l : list nat) (t : trace) : Prop :=*)
+  (*match l with*)
+  (*| [] => match t with*)
+           (*| [] => False*)
+           (*| In s :: t' => False*)
+           (*| Out s :: t' => s = 0 /\ t' = [In 0]*)
+           (*end*)
+  (*| x :: l' => match t with*)
+           (*| [] => False*)
+           (*| In s :: t' => False*)
+           (*| Out s :: t' => s = 0 /\ t' = [In 0]*)
+  (*end.*)
+(*| Ssn: forall s n x t,*)
+    (*sum_spec (Out s :: t ++ [In n])*)
+    (*-> sum_spec (Out (s + x) :: In x :: t ++ [In (S n)]).*)
+
+(*Example zero_sum : sum_spec [Out 0 ; In 0].*)
+(*Proof. econstructor. Qed.*)
+(*Example three_sum : sum_spec [Out 3 ; In 3 ; In 1].*)
+(*Proof.*)
+  (*eapply Ssn with (n := 0) (x := 3) (s := 0) (t := nil).*)
+  (*simplify.*)
+  (*econstructor 2.*)
+(*Qed.*)
